Verify try_mark

spanning.v
@@ -1,20 +1,26 @@
+From iris.algebra Require Import frac dec_agree.
+From iris.program_logic Require Export invariants ghost_ownership.
+From iris.program_logic Require Import ownership auth.
+From iris.proofmode Require Import weakestpre tactics.
 From iris.program_logic Require Export global_functor.
 From iris.proofmode Require Import invariants ghost_ownership.
 From iris.heap_lang Require Import proofmode notation.
+From iris.heap_lang Require Export lifting heap notation.
 From iris.heap_lang.lib Require Import par.
 Import uPred.
 
+From iris_spanning_tree Require Import graph mon.
+
 Definition try_mark : val :=
-  λ: "y",
-  let: "e" := ! "y" in CAS "y" (#false, Snd "e") (#true, Snd "e").
+  λ: "y", let: "e" := Fst (!"y") in CAS "e" #false #true.
 
 Definition unmark_fst : val :=
   λ: "y",
-  let: "e" := ! "y" in "y" <- (#true, (NONE, Snd (Snd "e"))).
+  let: "e" := ! "y" in "y" <- (Fst "e", (NONE, Snd (Snd "e"))).
 
 Definition unmark_snd : val :=
   λ: "y",
-  let: "e" := ! "y" in "y" <- (#true, (Fst (Snd "e"), NONE)).
+  let: "e" := ! "y" in "y" <- (Fst "e", (Fst (Snd "e"), NONE)).
 
 Definition span : val :=
   rec: "span" "x" :=
@@ -29,3 +35,101 @@ Definition span : val :=
     else
       #false
   end.
+
+  (* This change should happen in iris. -- to allow _ in the context with
+which we are binding. *)
+  Local Tactic Notation "wp_bind" open_constr(K) :=
+  lazymatch eval hnf in K with
+  | [] => idtac
+  | _ => etrans; [|fast_by apply (wp_bind K)]; simpl
+  end.
+
+  Ltac open_graph_inv Hinv key γ mr pat :=
+    let HIK := eval cbv in ("[" +:+ Hinv +:+ " " +:+ key +:+ "]") in
+    iDestruct (UnPack_later with HIK) as HIK;
+    [iNext; iSplitL key; by iFrame|];
+    rewrite {2}/graph_inv later_exist; iDestruct Hinv as (γ) Hinv;
+    rewrite later_exist; iDestruct Hinv as (mr) Hinv;
+    iDestruct Hinv as pat.
+
+
+Section Helpers.
+  Context {Σ} {Ih : heapG Σ} {Im : markingG Σ} {Ig : graphG Σ} {Ii : invtokG Σ}.
+
+  Lemma wp_try_mark g Mrk k q (x : loc) w :
+    marked g = ∅ →
+    (heap_ctx ★ graph_ctx g Mrk ★ Γρ(q, x [↦] w) ★ κ(k))
+      ⊢
+      WP (try_mark #x)
+      {{ v,
+         match v with
+         | # true =>
+           (∃ u, (w = None)
+                   ★ ((g !! x) = Some (false, u)) ★
+                   Γρ(q, x [↦] Excl' u))
+         | # false => Γρ(q, x [↦] w)
+         | _ => False
+         end
+           ★ μ(x) ★ κ(k)
+      }}.
+  Proof.
+    intros Hgnm. iIntros "(#Hheap & #Hgr & Hx & key)". unfold try_mark.
+    wp_let; wp_focus (! _)%E. unfold graph_ctx; iInv graphN as "Hinv".
+    open_graph_inv "Hinv" "key" γ mr "(Hi1 & Hi2 & Hi3 & Hi4 & Hi5)".
+    iDestruct (graph_open_later with "[Hx Hi1 Hi3 Hi5]") as
+        "(Hi1 & Hi3 & Hi5 & Hi6 & Hx)"; [by iFrame|].
+    rewrite later_exist. iDestruct "Hi6" as (u) "[Hi61 Hi62]".
+    rewrite later_exist. iDestruct "Hi62" as (m) "[Hi62 [Hi63 Hi64]]".
+    wp_load; iPvsIntro. iDestruct "Hi61" as %Hi61. iDestruct "Hi4" as %Hi4.
+    iDestruct "Hi1" as %Hi1. iDestruct "Hi62" as %Hi62.
+    iDestruct (graph_close with "[Hi3 Hi5 Hi63 Hi64 Hx]") as "(Hi1&Hi3&Hx)";
+      eauto. iFrame. iExists _; eauto. iSplitR; eauto. by iExists _; iFrame.
+    iSplitL "Hi1 Hi2 Hi3".
+    { iNext. iApply Pack. iExists _, _; iFrame. by iSplitL; iPureIntro. }
+    destruct u as [bu lu]; simpl. wp_focus (Fst _). iApply wp_fst; eauto.
+    { by destruct lu as [[] []]; simpl; eauto. }
+    iNext; iPvsIntro; wp_let. iInv graphN as "Hinv".
+    clear Hi4 Hi1 Hi61.
+    open_graph_inv "Hinv" "key" γ' mr' "(Hi1 & Hi2 & Hi3 & Hi4 & Hi5)".
+    iDestruct (graph_open_later with "[Hx Hi1 Hi3 Hi5]") as
+        "(Hi1 & Hi3 & Hi5 & Hi6 & Hx)"; [by iFrame|].
+    rewrite later_exist. iDestruct "Hi6" as (u) "[Hi61 Hi62]".
+    rewrite later_exist. iDestruct "Hi62" as (m') "[Hi62 [Hi63 Hi64]]".
+    iTimeless "Hi62". iDestruct "Hi62" as %Hi62'. rewrite Hi62' in Hi62.
+    iTimeless "Hi61". iDestruct "Hi61" as %Hi61.
+    iTimeless "Hi4". iDestruct "Hi4" as %Hi4.
+    iTimeless "Hi1". iDestruct "Hi1" as %Hi1.
+    inversion Hi62; subst; clear Hi62.
+    destruct u as [[] lu']; simpl in *.
+    - (* CAS fails *)
+      wp_cas_fail.
+      iDestruct (graph_close with "[Hi3 Hi5 Hi63 Hi64 Hx]") as "(Hi1&Hi3&Hx)";
+      eauto. iFrame. iExists _; eauto. iSplitR; eauto. by iExists _; iFrame.
+      iPvs (already_marked with "Hi2") as "[Hi2 Hxm]"; [|iFrame "Hxm"].
+      { rewrite Hi4. eapply graph.is_marked; eauto. }
+      iPvsIntro; iFrame. iNext; iApply Pack.
+      unfold graph_inv; iExists _, _; iFrame; by repeat iSplitL.
+    - (* CAS succeeds *)
+      wp_cas_suc. rewrite (graph_expose_node g γ' x (false, lu')) //=.
+      iDestruct (graph_pointsto_unmarked with "[Hi3 Hx]")
+        as "[Hi3 [Hx %]]"; try by iFrame. by rewrite lookup_delete.
+      subst.
+      iPvs (mark_update_graph _ _ _ (Excl lu') with "[Hi3 Hx]") as "[Hi3 Hx]";
+        try by iFrame. done. by rewrite lookup_delete.
+      iPvs (new_marked with "Hi2") as "[Hi2 Hm]". iFrame "key Hm".
+      erewrite mark_update_deleted.
+      iDestruct (graph_close with "[Hi3 Hi5 Hi63 Hi64 Hx]") as "(Hi1&Hi3&Hx)";
+        try iFrame.
+      { by apply mark_update_dom_stable. }
+      { iExists (_, _). iSplitR; [| iExists _; by iFrame].
+          by rewrite mark_update_lookup. }
+      iPvsIntro. iSplitR "Hx".
+      + iNext; iApply Pack; unfold graph_inv. iExists _, _; iFrame.
+        iSplit; iPureIntro.
+        { by rewrite new_marking_dom marking_union Hi4. }
+        { erewrite mark_update_dom_stable; eauto. }
+      + iExists _; iFrame. iSplit; iPureIntro; eauto using unmarked_from_g.
+  Qed.
+
+
+End Helpers.
